src/proofs/no_slashable_attestations/supporting_lemmas/ind_inv.dfy
@@ -332,7 +332,7 @@ module Att_Ind_Inv_With_Empty_Initial_Attestation_Slashing_DB
         process.dv_pubkey,
         dv.all_nodes
     )
-    requires quorum_constraints(dv)
+    requires inv_quorum_constraints(dv)
     requires attestation_share in dv.att_network.allMessagesSent
     requires pred_rcvd_attestation_shares_is_in_all_messages_sent_single_node_state(dv, process)
     requires forall a | a in process.bn.attestations_submitted :: exists hn', att_share: AttestationShare ::
@@ -490,7 +490,7 @@ module Att_Ind_Inv_With_Empty_Initial_Attestation_Slashing_DB
         process.dv_pubkey,
         dv.all_nodes
     )
-    requires quorum_constraints(dv)
+    requires inv_quorum_constraints(dv)
     requires attestation_share in dv.att_network.allMessagesSent
     requires pred_rcvd_attestation_shares_is_in_all_messages_sent_single_node_state(dv, process)
     // requires forall a | a in process.bn.attestations_submitted :: exists hn', att_share: AttestationShare ::
@@ -751,9 +751,9 @@ module Att_Ind_Inv_With_Empty_Initial_Attestation_Slashing_DB
         s.dv_pubkey,
         s.all_nodes
     )
-    requires only_dv_construct_signed_attestation_signature(s)  
+    requires inv_only_dv_construct_signed_attestation_signature(s)  
     requires invNetwork(s)
-    requires quorum_constraints(s)
+    requires inv_quorum_constraints(s)
     requires pred_rcvd_attestation_shares_is_in_all_messages_sent(s)    
     ensures pred_4_1_b(s')
     {
@@ -1006,9 +1006,9 @@ module Att_Ind_Inv_With_Empty_Initial_Attestation_Slashing_DB
     requires NextEvent(s, event, s')  
     requires pred_4_1_c(s)
     requires pred_4_1_f_b(s)
-    requires quorum_constraints(s)
+    requires inv_quorum_constraints(s)
     requires inv53(s)
-    requires only_dv_construct_signed_attestation_signature(s)
+    requires inv_only_dv_construct_signed_attestation_signature(s)
     requires |s.all_nodes| > 0
     requires s'.att_network.allMessagesSent == s.att_network.allMessagesSent + 
                             getMessagesFromMessagesWithRecipient({});
@@ -1065,10 +1065,10 @@ module Att_Ind_Inv_With_Empty_Initial_Attestation_Slashing_DB
     requires pred_4_1_c(s)
     requires pred_4_1_f_b(s)
     requires inv_attestation_shares_to_broadcast_is_a_subset_of_all_messages_sent(s)  
-    requires quorum_constraints(s)
-    requires unchanged_honesty(s)
+    requires inv_quorum_constraints(s)
+    requires inv_unchanged_honesty(s)
     requires inv53(s)
-    requires only_dv_construct_signed_attestation_signature(s)
+    requires inv_only_dv_construct_signed_attestation_signature(s)
     requires pred_4_1_f_a(s)    
     requires pred_4_1_g_i(s)
     requires pred_4_1_g_i_for_dvc(s)          
@@ -1151,8 +1151,8 @@ module Att_Ind_Inv_With_Empty_Initial_Attestation_Slashing_DB
     requires NextEvent(s, event, s')  
     requires event.HonestNodeTakingStep?
     requires event.event.AttConsensusDecided?
-    requires quorum_constraints(s)
-    requires unchanged_honesty(s)        
+    requires inv_quorum_constraints(s)
+    requires inv_unchanged_honesty(s)        
     requires |s.all_nodes| > 0    
     ensures s'.consensus_on_attestation_data[event.event.id].decided_value.safe_get() == event.event.decided_attestation_data; 
     {
@@ -1217,10 +1217,10 @@ module Att_Ind_Inv_With_Empty_Initial_Attestation_Slashing_DB
     requires pred_4_1_c(s)
     requires pred_4_1_f_b(s)
     requires inv_attestation_shares_to_broadcast_is_a_subset_of_all_messages_sent(s)  
-    requires quorum_constraints(s)
-    requires unchanged_honesty(s)
+    requires inv_quorum_constraints(s)
+    requires inv_unchanged_honesty(s)
     requires inv53(s)
-    requires only_dv_construct_signed_attestation_signature(s)
+    requires inv_only_dv_construct_signed_attestation_signature(s)
     requires pred_4_1_f_a(s)    
     requires pred_4_1_g_i(s)
     requires pred_4_1_g_i_for_dvc(s)          
@@ -1305,10 +1305,10 @@ module Att_Ind_Inv_With_Empty_Initial_Attestation_Slashing_DB
     requires pred_4_1_c(s)
     requires pred_4_1_f_b(s)
     requires inv_attestation_shares_to_broadcast_is_a_subset_of_all_messages_sent(s)  
-    requires quorum_constraints(s)
-    requires unchanged_honesty(s)
+    requires inv_quorum_constraints(s)
+    requires inv_unchanged_honesty(s)
     requires inv53(s)
-    requires only_dv_construct_signed_attestation_signature(s)
+    requires inv_only_dv_construct_signed_attestation_signature(s)
     requires pred_4_1_f_a(s)    
     requires pred_4_1_g_i(s)
     requires pred_4_1_g_i_for_dvc(s)          
@@ -1393,9 +1393,9 @@ module Att_Ind_Inv_With_Empty_Initial_Attestation_Slashing_DB
     requires pred_4_1_c(s)
     requires pred_4_1_f_b(s)
     requires inv_attestation_shares_to_broadcast_is_a_subset_of_all_messages_sent(s)  
-    requires quorum_constraints(s)
+    requires inv_quorum_constraints(s)
     requires inv53(s)
-    requires only_dv_construct_signed_attestation_signature(s)
+    requires inv_only_dv_construct_signed_attestation_signature(s)
     requires |s.all_nodes| > 0
     ensures pred_4_1_c(s') 
     {
@@ -1458,10 +1458,10 @@ module Att_Ind_Inv_With_Empty_Initial_Attestation_Slashing_DB
     )
     requires NextEventPreCond(s, event)
     requires NextEvent(s, event, s')  
-    requires quorum_constraints(s)
-    requires unchanged_honesty(s)
+    requires inv_quorum_constraints(s)
+    requires inv_unchanged_honesty(s)
     requires inv53(s)
-    requires only_dv_construct_signed_attestation_signature(s)
+    requires inv_only_dv_construct_signed_attestation_signature(s)
     requires pred_4_1_c(s)
     requires pred_4_1_f_b(s)
     requires inv_attestation_shares_to_broadcast_is_a_subset_of_all_messages_sent(s)      
@@ -1585,9 +1585,9 @@ module Att_Ind_Inv_With_Empty_Initial_Attestation_Slashing_DB
     requires NextEvent(s, event, s')  
     requires event.HonestNodeTakingStep?
     requires cid in s'.consensus_on_attestation_data.Keys
-    requires quorum_constraints(s)
+    requires inv_quorum_constraints(s)
     requires inv53(s)
-    requires only_dv_construct_signed_attestation_signature(s)
+    requires inv_only_dv_construct_signed_attestation_signature(s)
     requires pred_4_1_f_a(s)    
     requires s.consensus_on_attestation_data[cid].decided_value.isPresent()
     ensures is_a_valid_decided_value(s'.consensus_on_attestation_data[cid]); 
@@ -1702,9 +1702,9 @@ module Att_Ind_Inv_With_Empty_Initial_Attestation_Slashing_DB
     )
     requires NextEventPreCond(s, event)
     requires NextEvent(s, event, s')  
-    requires quorum_constraints(s)
+    requires inv_quorum_constraints(s)
     requires inv53(s)
-    requires only_dv_construct_signed_attestation_signature(s)
+    requires inv_only_dv_construct_signed_attestation_signature(s)
     requires pred_4_1_f_a(s)    
     ensures pred_4_1_f_a(s')   
     {
@@ -1752,9 +1752,9 @@ module Att_Ind_Inv_With_Empty_Initial_Attestation_Slashing_DB
     )
     requires pred_4_1_f_a(s)    
     requires pred_4_1_g_i(s)
-    requires quorum_constraints(s)
-    requires unchanged_honesty(s)
-    requires only_dv_construct_signed_attestation_signature(s)
+    requires inv_quorum_constraints(s)
+    requires inv_unchanged_honesty(s)
+    requires inv_only_dv_construct_signed_attestation_signature(s)
     requires cid in s.consensus_on_attestation_data.Keys
     requires s.consensus_on_attestation_data[cid].decided_value.isPresent()
     ensures s.consensus_on_attestation_data[cid].decided_value.safe_get().slot == cid
@@ -1793,14 +1793,14 @@ module Att_Ind_Inv_With_Empty_Initial_Attestation_Slashing_DB
     requires pred_4_1_f_a(s)    
     requires pred_4_1_g_i(s)
     requires pred_4_1_g_i_for_dvc(s)  
-    requires quorum_constraints(s)
-    requires unchanged_honesty(s)
-    requires only_dv_construct_signed_attestation_signature(s)  
+    requires inv_quorum_constraints(s)
+    requires inv_unchanged_honesty(s)
+    requires inv_only_dv_construct_signed_attestation_signature(s)  
     ensures pred_4_1_f_b(s') 
     {
-        lemma_quorum_constraints_dv_next(s, event, s');
-        lemma_unchanged_honesty_dv_next(s, event, s');
-        lemma_only_dv_construct_signed_attestation_signature_dv_next(s, event, s');
+        lemma_inv_quorum_constraints_dv_next(s, event, s');
+        lemma_inv_unchanged_honesty_dv_next(s, event, s');
+        lemma_inv_only_dv_construct_signed_attestation_signature_dv_next(s, event, s');
         lemma_pred_4_1_f_a(s, event, s');
         lemma_pred_4_1_f_g_i(s, event, s');
         lemma_pred_4_1_f_b2(s');   
@@ -1811,9 +1811,9 @@ module Att_Ind_Inv_With_Empty_Initial_Attestation_Slashing_DB
     )
     requires pred_4_1_f_a(s)    
     requires pred_4_1_g_i(s)
-    requires quorum_constraints(s)
-    requires unchanged_honesty(s)
-    requires only_dv_construct_signed_attestation_signature(s)
+    requires inv_quorum_constraints(s)
+    requires inv_unchanged_honesty(s)
+    requires inv_only_dv_construct_signed_attestation_signature(s)
     ensures pred_4_1_f_b(s) 
     {
         forall cid |
@@ -1871,9 +1871,9 @@ module Att_Ind_Inv_With_Empty_Initial_Attestation_Slashing_DB
     )   returns (attestation_duty: AttestationDuty, attestation_slashing_db: set<SlashingDBAttestation>)
     requires NextEventPreCond(s, event)
     requires NextEvent(s, event, s')    
-    requires quorum_constraints(s)
-    requires unchanged_honesty(s)
-    requires only_dv_construct_signed_attestation_signature(s)      
+    requires inv_quorum_constraints(s)
+    requires inv_unchanged_honesty(s)
+    requires inv_only_dv_construct_signed_attestation_signature(s)      
     requires
             && hn in s'.consensus_on_attestation_data[cid].honest_nodes_validity_functions.Keys
             && vp in s'.consensus_on_attestation_data[cid].honest_nodes_validity_functions[hn]
@@ -1960,9 +1960,9 @@ module Att_Ind_Inv_With_Empty_Initial_Attestation_Slashing_DB
     requires NextEventPreCond(s, event)
     requires NextEvent(s, event, s')    
     requires pred_4_1_g_i(s)
-    requires quorum_constraints(s)
-    requires unchanged_honesty(s)
-    requires only_dv_construct_signed_attestation_signature(s)      
+    requires inv_quorum_constraints(s)
+    requires inv_unchanged_honesty(s)
+    requires inv_only_dv_construct_signed_attestation_signature(s)      
     requires pred_4_1_g_i_for_dvc(s)  
     ensures pred_4_1_g_i(s')   
     {
@@ -2347,9 +2347,9 @@ module Att_Ind_Inv_With_Empty_Initial_Attestation_Slashing_DB
     )   
     requires NextEventPreCond(s, event)
     requires NextEvent(s, event, s')    
-    requires quorum_constraints(s)
-    requires unchanged_honesty(s)
-    requires only_dv_construct_signed_attestation_signature(s)      
+    requires inv_quorum_constraints(s)
+    requires inv_unchanged_honesty(s)
+    requires inv_only_dv_construct_signed_attestation_signature(s)      
     requires pred_4_1_g_i_for_dvc(s)  
     ensures pred_4_1_g_i_for_dvc(s')    
     {
@@ -2441,9 +2441,9 @@ module Att_Ind_Inv_With_Empty_Initial_Attestation_Slashing_DB
     //     s': DVState
     // )   
     // requires NextEvent(s, event, s') 
-    // requires quorum_constraints(s)
-    // requires unchanged_honesty(s)
-    // requires only_dv_construct_signed_attestation_signature(s)      
+    // requires inv_quorum_constraints(s)
+    // requires inv_unchanged_honesty(s)
+    // requires inv_only_dv_construct_signed_attestation_signature(s)      
     // requires inv_g_a(s)  
     // // ensures pred_4_1_g_iii(s')      
     // {
@@ -2639,9 +2639,9 @@ module Att_Ind_Inv_With_Empty_Initial_Attestation_Slashing_DB
     //     s': DVState
     // )   
     // requires NextEvent(s, event, s') 
-    // requires quorum_constraints(s)
-    // requires unchanged_honesty(s)
-    // requires only_dv_construct_signed_attestation_signature(s)      
+    // requires inv_quorum_constraints(s)
+    // requires inv_unchanged_honesty(s)
+    // requires inv_only_dv_construct_signed_attestation_signature(s)      
     // requires inv_g_c(s)  
     // // ensures pred_4_1_g_iii(s')      
     // {
@@ -3289,8 +3289,8 @@ module Att_Ind_Inv_With_Empty_Initial_Attestation_Slashing_DB
     requires NextEvent(s, event, s')    
     requires pred_4_1_g_iii(s)
     requires invNetwork(s)
-    requires quorum_constraints(s)
-    requires only_dv_construct_signed_attestation_signature(s)
+    requires inv_quorum_constraints(s)
+    requires inv_only_dv_construct_signed_attestation_signature(s)
     requires inv53(s)
     ensures forall ci: nat ::
             var s_consensus := s.consensus_on_attestation_data[ci];
@@ -3334,8 +3334,8 @@ module Att_Ind_Inv_With_Empty_Initial_Attestation_Slashing_DB
     requires NextEventPreCond(s, event)
     requires NextEvent(s, event, s')  
     requires invNetwork(s)
-    requires quorum_constraints(s)
-    requires only_dv_construct_signed_attestation_signature(s)
+    requires inv_quorum_constraints(s)
+    requires inv_only_dv_construct_signed_attestation_signature(s)
     requires inv53(s)
     requires s.consensus_on_attestation_data[ci].decided_value.isPresent()
     ensures 
@@ -3374,8 +3374,8 @@ module Att_Ind_Inv_With_Empty_Initial_Attestation_Slashing_DB
     requires NextEvent(s, event, s')  
     requires pred_4_1_g_iii(s)
     requires invNetwork(s)
-    requires quorum_constraints(s)
-    requires only_dv_construct_signed_attestation_signature(s)
+    requires inv_quorum_constraints(s)
+    requires inv_only_dv_construct_signed_attestation_signature(s)
     requires inv53(s)  
     ensures inv_g_iii_body_body(s', s_node)  
     {
@@ -3409,8 +3409,8 @@ module Att_Ind_Inv_With_Empty_Initial_Attestation_Slashing_DB
     requires NextEvent(s, event, s')  
     requires pred_4_1_g_iii(s)
     requires invNetwork(s)
-    requires quorum_constraints(s)
-    requires only_dv_construct_signed_attestation_signature(s)
+    requires inv_quorum_constraints(s)
+    requires inv_only_dv_construct_signed_attestation_signature(s)
     requires inv53(s)  
     ensures inv_g_b_body_body_new(s', n, s_node)  
     {
@@ -3456,8 +3456,8 @@ module Att_Ind_Inv_With_Empty_Initial_Attestation_Slashing_DB
     requires NextEvent(s, event, s')  
     requires pred_4_1_g_iii(s)
     requires invNetwork(s)
-    requires quorum_constraints(s)
-    requires only_dv_construct_signed_attestation_signature(s)
+    requires inv_quorum_constraints(s)
+    requires inv_only_dv_construct_signed_attestation_signature(s)
     requires inv53(s)  
     ensures inv_g_d_a_body_body(s', n, s_node)  
     {
@@ -3511,8 +3511,8 @@ module Att_Ind_Inv_With_Empty_Initial_Attestation_Slashing_DB
 
     // requires pred_4_1_g_iii(s)
     // requires invNetwork(s)
-    // requires quorum_constraints(s)
-    // requires only_dv_construct_signed_attestation_signature(s)
+    // requires inv_quorum_constraints(s)
+    // requires inv_only_dv_construct_signed_attestation_signature(s)
     // requires inv53(s)  
     // ensures inv_g_iii_body_body(s', s_node)  
     {
@@ -3535,8 +3535,8 @@ module Att_Ind_Inv_With_Empty_Initial_Attestation_Slashing_DB
     requires NextEvent(s, event, s')  
     requires event.HonestNodeTakingStep?
     requires event.event.AttConsensusDecided?
-    requires quorum_constraints(s)
-    requires only_dv_construct_signed_attestation_signature(s)
+    requires inv_quorum_constraints(s)
+    requires inv_only_dv_construct_signed_attestation_signature(s)
     requires inv53(s)    
     ensures s'.consensus_on_attestation_data[event.event.id].decided_value.isPresent(); 
     ensures  s'.consensus_on_attestation_data[event.event.id].decided_value.safe_get() == event.event.decided_attestation_data;    
@@ -3579,9 +3579,9 @@ module Att_Ind_Inv_With_Empty_Initial_Attestation_Slashing_DB
     requires NextEvent(s, event, s')  
     requires event.HonestNodeTakingStep?
     requires event.event.AttConsensusDecided?
-    requires quorum_constraints(s)
-    requires unchanged_honesty(s)
-    requires only_dv_construct_signed_attestation_signature(s)
+    requires inv_quorum_constraints(s)
+    requires inv_unchanged_honesty(s)
+    requires inv_only_dv_construct_signed_attestation_signature(s)
     requires inv53(s)    
     requires pred_4_1_f_a(s)    
     requires pred_4_1_g_i(s)
@@ -3611,9 +3611,9 @@ module Att_Ind_Inv_With_Empty_Initial_Attestation_Slashing_DB
             s.all_nodes
         )
         && invNetwork(s)
-        && quorum_constraints(s)
-        && unchanged_honesty(s)
-        && only_dv_construct_signed_attestation_signature(s)
+        && inv_quorum_constraints(s)
+        && inv_unchanged_honesty(s)
+        && inv_only_dv_construct_signed_attestation_signature(s)
         && inv53(s)
         && pred_4_1_g_iii_a(s)
         && pred_4_1_g_iii_a_a(s)
